src/sf_proof.v
@@ -4,6 +4,8 @@ Require Import RelDec.
 Require Import List.
 Require Import Sorted.
 Require Import Permutation.
+Require Import FunctionalExtensionality.
+Require Import Classical.
 Import ListNotations.
 
 
@@ -13,28 +15,92 @@ Variable candidate : Set.
 Variable reldec_candidate : RelDec (@eq candidate).
 Variable reldec_correct_candidate : RelDec_Correct reldec_candidate.
 
+Hint Resolve reldec_correct_candidate: rcv.
+
 Definition in_record (rec : sf_imp.record candidate) (c : candidate) :=
 exists e, In e rec /\ In c e.
 
-Lemma no_viable_candidates_correct : 
-forall rec bal,
-sf_imp.no_viable_candidates candidate _ rec bal = true -> 
-sf_spec.no_viable_candidates candidate (in_record rec) bal.
+Hint Rewrite Forall_forall : rcv.
+Hint Rewrite forallb_forall : rcv.
+Hint Rewrite existsb_exists : rcv.
+Hint Rewrite Bool.negb_true_iff : rcv.
+Hint Rewrite Bool.negb_false_iff : rcv.
+Hint Rewrite <- @neg_rel_dec_correct : rcv.
+
+Ltac arw := try autorewrite with rcv in *.
+
+
+Ltac unfold_defs := cbv [sf_imp.no_viable_candidates sf_spec.no_viable_candidates
+                         sf_imp.eliminated sf_imp.no_viable_candidates_selection
+                        in_record sf_spec.overvote sf_spec.properly_selects
+                        sf_spec.does_not_select eq_dec sf_spec.selected_candidate
+                        sf_spec.continuing_ballot sf_spec.exhausted_ballot].
+
+Ltac unfold_defs_star := cbv [sf_imp.no_viable_candidates sf_spec.no_viable_candidates
+                         sf_imp.eliminated sf_imp.no_viable_candidates_selection in_record 
+                         sf_spec.overvote sf_spec.properly_selects
+                         sf_spec.does_not_select eq_dec sf_spec.selected_candidate
+                         sf_spec.continuing_ballot sf_spec.exhausted_ballot] in *.
+
+
+Tactic Notation "unfold_defs" "in" "*" := unfold_defs_star.
+
+Ltac copy H :=
+match type of H with 
+?P => assert P by exact H end.
+
+Ltac destruct_exists :=
+repeat
+match goal with
+| [ H : exists _, _ |- _ ] => destruct H
+end.
+
+Ltac intuitione :=
+repeat (destruct_exists; intuition).
+
+
+Ltac dlp := try
+        match goal with
+        | [ H : context[ let (a, b) := ?X in _ ] |- _ ] => destruct X eqn:?
+        end.
+
+
+Ltac inv H := inversion H; subst; clear H.
+
+Ltac notHyp P :=
+  match goal with
+    | [ _ : P |- _ ] => fail 1
+    | _ =>
+      match P with
+        | ?P1 /\ ?P2 => first [ notHyp P1 | notHyp P2 | fail 2 ]
+        | _ => idtac
+      end
+  end.
+
+Ltac extend pf :=
+  let t := type of pf in
+    notHyp t; generalize pf; intro.
+
+Ltac completer :=
+  repeat match goal with
+           | [ |- _ /\ _ ] => constructor
+           | [ H : _ /\ _ |- _ ] => destruct H
+           | [ H : ?P -> ?Q, H' : ?P |- _ ] => specialize (H H')
+           | [ |- forall x, _ ] => intro
+           | [ H : forall x, ?P x -> _, H' : ?P ?X |- _ ] => extend (H X H')
+         (*  | [ H : forall (x : ?P), _, H' : ?P |- _ ] => extend (H H')*)
+         end.
+
+Lemma forallb_false_exists :
+forall  {A} p (a : list A),
+forallb p a = false ->
+exists x, In x a /\ p x = false.
 Proof.
-intros.
-unfold sf_imp.no_viable_candidates in *. rewrite forallb_forall in H.
-unfold sf_spec.no_viable_candidates.
-intros.
-specialize (H _ H0). unfold sf_imp.no_viable_candidates_selection in *.
-rewrite forallb_forall in H. apply H in H1.
-unfold sf_imp.eliminated in H1.
-rewrite existsb_exists in H1.
-destruct H1.
-unfold in_record. destruct H1.
-rewrite existsb_exists in H2. destruct H2.
-destruct H2. 
-apply reldec_correct_candidate in H3. subst.
-exists x. auto.
+intros. induction a.
+inv H.
+simpl in H. rewrite Bool.andb_false_iff in *.
+destruct H. exists a. intuition.
+intuition. destruct H0.  exists x. simpl. intuition.
 Qed.
 
 Lemma existsb_false_forall :
@@ -52,25 +118,76 @@ induction l.
   + intuition.
 Qed.
 
+Ltac intuition_nosplit :=
+repeat
+match goal with
+| [ H : _ /\ _ |- _ ] => destruct H
+| [ H : False |- _] => inv H
+| [ H : In _ [] |- _] => inv H
+| [ H : eq_dec _ _ = true |- _] => apply reldec_correct_candidate in H; subst
+| [ |- eq_dec _ _ = true ] => apply reldec_correct_candidate 
+| [ H : _ ?[ eq ] _ = true |- _] => apply reldec_correct_candidate in H; subst
+| [|-  _ ?[ eq ] _ = true ] => apply reldec_correct_candidate; subst
+| [ H : existsb _ _ = false |- _] => apply existsb_false_forall in H
+| [ H : forallb _ _ = false |- _] => apply forallb_false_exists in H
+| [ H : (_, _) = (_, _) |- _] => inv H
+| [ H : Some _ = Some _ |- _] => inv H
+| [ |- ~_ ] => intro
+| [ H :  sf_spec.next_ranking _ _ [] _ |- _ ] => inv H
+end.
+
+Ltac unique :=
+repeat match goal with
+| [ H : sf_spec.next_ranking _ _ _ ?x, H' : sf_spec.next_ranking _ _ _ ?y |- _ ] =>
+  first [ assert (x = y) as Trash by auto ; clear Trash | 
+          extend (sf_spec.next_ranking_unique _ _ _ _ _ H H')]
+end.
+
+Ltac destruct_ifs :=
+repeat
+match goal with
+| [ H : context[ if ?b then _ else _ ] |- _] => destruct b eqn:?
+end. 
+
+
+Ltac solve_rcv' := repeat (intros; unfold_defs in *; arw; destruct_exists; 
+                           destruct_ifs; intuition_nosplit; completer; dlp; try subst;
+                           try solve [simpl in *; eauto with rcv]; 
+                          try solve [simpl in *; congruence]).
+
+
+Ltac solve_rcv := 
+match goal with
+| [ |- _ /\ _] => split; solve_rcv'; []
+| _ => solve_rcv'
+end.
+
+
+
+Lemma no_viable_candidates_correct : 
+forall rec bal,
+sf_imp.no_viable_candidates candidate _ rec bal = true -> 
+sf_spec.no_viable_candidates candidate (in_record rec) bal.
+Proof.
+solve_rcv.  
+specialize (H _ H0). solve_rcv.  
+apply H in H1.
+solve_rcv. 
+Qed.
+
+
+
 Lemma eliminated_correct :
 forall rec can,
 sf_imp.eliminated candidate _ rec can = true <->
 in_record rec can.
 Proof.
-split.
-intros.
-unfold sf_imp.eliminated in *. rewrite existsb_exists in H.
-destruct H; intuition.
-rewrite existsb_exists in H1. destruct H1; intuition.
-unfold in_record.
-apply reldec_correct_candidate in H2. subst; eauto.
-intros.
-unfold sf_imp.eliminated in *. rewrite existsb_exists.
-unfold in_record in H. destruct H. exists x. intuition.
-rewrite existsb_exists. exists can. intuition.
-apply reldec_correct_candidate. auto.
+split; solve_rcv.
+ exists x. solve_rcv. intuition.
+ exists can.  solve_rcv. 
 Qed.
 
+(*
 Definition no_viable_candidates eliminated (b : sf_spec.ballot candidate) :=
 Forall (Forall eliminated) b.
 
@@ -87,74 +204,97 @@ specialize (H rank). rewrite Forall_forall in H.
 intuition.
 rewrite Forall_forall. intro. rewrite Forall_forall. intuition.
 specialize (H x). intuition.
+Qed.*)
+
+Ltac force_specialize P :=
+repeat
+match goal with
+| [ H : _ |- _] => extend (P H)
+end. 
+
+Ltac force_specialize_all :=
+repeat
+match goal with
+| [ H : (forall x, _) |- _ ] => progress (force_specialize H)
+end.
+
+
+
+Lemma next_ranking_not_overvote :
+forall rec bal cd bal' a,
+sf_imp.next_ranking candidate _ rec (a :: bal) = Some (cd, bal') ->
+~sf_spec.overvote candidate a.
+Proof.
+intros. intro.
+simpl in *. 
+destruct a; solve_rcv;
+force_specialize_all;
+simpl in *; intuition; subst; solve_rcv.
 Qed.
+
+Lemma next_ranking_selects : forall a bal cd bal' rec,
+    sf_imp.next_ranking candidate reldec_candidate rec (a :: bal) =
+    Some (cd, bal') ->
+    sf_spec.does_not_select candidate (in_record rec) a ->
+    sf_imp.next_ranking candidate reldec_candidate rec (bal) = Some (cd, bal').
+Proof.
+intros.
+destruct a; simpl in *; solve_rcv.
+destruct H0; solve_rcv.
+assert (x=cd).
+simpl in H0; intuition; force_specialize_all; solve_rcv.
+subst. clear H0. 
+force_specialize_all; solve_rcv.
+force_specialize_all; solve_rcv. 
+Qed. 
+                            
+Hint Resolve next_ranking_not_overvote : rcv.
 
 Lemma next_ranking_correct :
 forall rec bal cd bal' ,
 sf_imp.next_ranking candidate _ rec bal = Some (cd, bal') ->
-exists l,(sf_spec.next_ranking candidate (in_record rec) bal l /\ Forall (eq cd) l).
+exists h t,(sf_spec.next_ranking candidate (in_record rec) bal (h::t) /\ Forall (eq cd) (h::t)).
 Proof.
 intros.
 induction bal.
-- simpl in *. congruence.
-- simpl in *.
-  destruct a.
-  + intuition. destruct H0. exists x. firstorder.
-  + destruct (forallb (eq_dec c) a) eqn:Heqb0.
-    * { destruct (sf_imp.eliminated candidate reldec_candidate rec c) eqn:?.
-         - apply IHbal in H. clear IHbal.
-           destruct H. destruct H. exists x.
-           split. left. intuition.
-           + intros.
-             assert (c = c0).
-             destruct H1. auto.
-             rewrite forallb_forall in Heqb0.
-             apply Heqb0 in H1.
-             apply reldec_correct_candidate in H1. auto.
-             subst.
-             unfold sf_imp.eliminated in Heqb. rewrite existsb_exists in Heqb.
-             destruct Heqb. intuition. rewrite existsb_exists in *. destruct H4.
-             destruct H2. apply reldec_correct_candidate in H4. subst.
-             unfold in_record. eauto.               
-           + intuition.
-         - inversion H. subst. clear H. 
-           exists (cd :: a).
-           split. right.
-           split.
-           + unfold sf_imp.eliminated in *. 
-             apply existsb_false_forall in Heqb.
-             rewrite forallb_forall in Heqb.
-             exists cd.
-             split.
-             * constructor. auto.
-             * intro. unfold in_record in *.
-               destruct H. destruct H. specialize (Heqb x H).
-               rewrite Bool.negb_true_iff in Heqb.
-               apply existsb_false_forall in Heqb.
-               rewrite forallb_forall in Heqb.
-               specialize (Heqb cd). intuition.
-               rewrite Bool.negb_true_iff in H1.
-               assert (cd = cd) by reflexivity.
-               apply reldec_correct_candidate in H2.
-               unfold eq_dec in *.
-               congruence.
-           + reflexivity.
-           + rewrite forallb_forall in Heqb0. rewrite Forall_forall. 
-             intuition. destruct H. auto. apply Heqb0 in H. apply reldec_correct_candidate.
-             auto.                                                                     
-      } 
-    * congruence.       
+- solve_rcv. 
+- solve_rcv.
+  destruct (sf_spec.ranking_cases _  (in_record rec) a); [ | destruct H0].
+  + apply next_ranking_not_overvote in H. intuition.
+  + solve_rcv. destruct a; simpl in *; solve_rcv. 
+    * { destruct H1. 
+        - exfalso. apply H2.
+          subst. exists x2. auto.
+        - exists x0; exists (x1); solve_rcv.
+          + constructor; solve_rcv.
+            * exists x2. split; auto. 
+              destruct H7. subst; auto.
+              force_specialize_all; solve_rcv.
+            * force_specialize_all; solve_rcv.
+      }
+    * { destruct H1. 
+        - subst. exists x. exists a. solve_rcv.
+          eapply sf_spec.next_ranking_valid; solve_rcv.
+        - exists cd.  exists a. 
+          solve_rcv. eapply sf_spec.next_ranking_valid; solve_rcv.
+          simpl in H1. intuition.
+          force_specialize_all; solve_rcv.
+      }
+  + apply next_ranking_selects in H; auto.
+    solve_rcv.
+    exists x; solve_rcv. exists x0.
+    destruct H0; solve_rcv. constructor; solve_rcv. 
+    constructor; solve_rcv. force_specialize_all; solve_rcv.
+    force_specialize_all; solve_rcv.
 Qed.
-
-
+ 
 Lemma next_ranking_in :
 forall e bal x,
   sf_spec.next_ranking candidate e bal x ->
   In x bal.
 Proof.
-induction bal; intros.
-- simpl in H. auto.
-- simpl in *. intuition.
+induction bal; solve_rcv.
+inv H; solve_rcv. 
 Qed.
 
 Lemma next_ranking_cons_or :
@@ -162,11 +302,14 @@ forall b1 bal e x,
 sf_spec.next_ranking candidate e (b1 :: bal) x ->
 sf_spec.next_ranking candidate e [b1] x \/ 
 sf_spec.next_ranking candidate e bal x.
-intros. simpl in  H. intuition. destruct H. destruct H.
-left. unfold sf_spec.next_ranking. right. eauto.
+intros. inv H; solve_rcv. left.
+destruct H4; solve_rcv. eapply sf_spec.next_ranking_valid; solve_rcv.
+left. eauto. eapply sf_spec.next_ranking_valid; solve_rcv.
 Qed.
 
-Ltac inv H := inversion H; subst; clear H.
+
+(* These don't have meaning anymore now that overvote is a ranking
+   level predicate 
 
 Lemma overvote_cons_or :
 forall b1 bal e ,
@@ -245,7 +388,7 @@ induction bal.
             specialize (Heqb _ H1). apply reldec_correct_candidate in Heqb. auto.
             auto. } 
     * congruence.
-Qed.
+Qed. *)
     
 Lemma no_viable_candidates_cons :
 forall a b e,
@@ -291,23 +434,25 @@ induction bal; intros.
 Qed.
   
 
+
+
 Lemma next_ranking_selected :
 forall bal cd bal' rec,
 sf_imp.next_ranking candidate _ rec bal = Some (cd, bal') ->
 sf_spec.selected_candidate candidate (in_record rec) bal cd.
-split.
-intros.
-unfold sf_spec.selected_candidate. 
-- unfold sf_spec.continuing_ballot. intro. 
-  unfold sf_spec.exhausted_ballot in H0.
-  destruct H0. 
-  + apply next_ranking_viable in H. auto.
-  + eapply next_ranking_not_overvote in H0; eauto.
-- apply next_ranking_correct in H. destruct H. destruct H.
-  exists x. intuition.
-  destruct x. induction bal. inv H. simpl in *. intuition. subst. 
-  destruct H; intuition.
-  inv H0. simpl in *. auto.
+solve_rcv.
+- destruct H0.
+ + apply H0; clear H0.
+   apply next_ranking_correct in H. 
+   solve_rcv.
+ + destruct bal; solve_rcv.
+   copy H.
+   apply next_ranking_correct in H. solve_rcv.
+   unique; subst.
+   force_specialize_all; solve_rcv. 
+- apply next_ranking_correct in H; solve_rcv.
+  exists (x :: x0); solve_rcv.  simpl in *.
+  force_specialize_all; solve_rcv; intuition.
 Qed.
 
 Lemma next_ranking_eliminated :
@@ -315,32 +460,35 @@ forall bal rec,
 sf_imp.next_ranking candidate _ rec bal = None ->
 sf_spec.exhausted_ballot candidate (in_record rec) bal.
 Proof.
-intros.
-unfold sf_spec.exhausted_ballot.
+intros. 
 induction bal.
--  left. unfold sf_spec.no_viable_candidates. intros. inv H0.
-- simpl in *. destruct a.
-   + intuition. left. apply no_viable_candidates_cons. intuition.
-     unfold sf_spec.no_viable_candidates. intros. inv H0; firstorder.
-     right. unfold sf_spec.overvote in *. destruct H1. exists x.
-     intuition. simpl. intuition.
-   + destruct (forallb (eq_dec c) a) eqn:?.
-     destruct (sf_imp.eliminated candidate reldec_candidate rec c) eqn:?; try congruence.
-     rewrite eliminated_correct in *.  
-     intuition. 
-     * left. unfold sf_spec.no_viable_candidates. intros. simpl in *. destruct H0.  
-       assert (candidate0 = c); subst; auto. rewrite forallb_forall in Heqb.
-       specialize (Heqb candidate0). simpl in H2. destruct H2; auto.
-       specialize (Heqb H0). apply reldec_correct_candidate in Heqb. auto.
-       unfold sf_spec.no_viable_candidates in *.
-       eapply H1; eauto.
-     * right. clear H Heqb0.
-       unfold sf_spec.overvote in *. 
-       destruct H1. intuition. destruct H1. destruct H. intuition.
-       exists x. simpl. intuition. left. intuition.
-       subst.
-       rewrite forallb_forall in Heqb. specialize (Heqb x0). 
-Admitted.
+- left. solve_rcv. 
+- simpl in *. destruct a; solve_rcv. 
+  + destruct IHbal; solve_rcv.
+    * left. intro. apply H0. solve_rcv.
+      exists x. inv H1; solve_rcv.
+    * right. exists x. solve_rcv. constructor; solve_rcv.
+  + destruct IHbal. 
+    * left. intro. apply H2; solve_rcv.
+      { inv H3. 
+        - solve_rcv.
+        - destruct H8; solve_rcv.  
+          + exfalso. simpl in *. repeat (intuition; subst); force_specialize_all; solve_rcv.
+          + inv H6; solve_rcv. 
+            * exfalso. apply H3. clear H3. exists x; solve_rcv.
+            * force_specialize_all. solve_rcv.
+              exfalso. apply H3; solve_rcv.
+      }
+    * right. solve_rcv. 
+      exists x1; solve_rcv.
+      constructor; solve_rcv. exists x; inv H6; force_specialize_all; solve_rcv.
+      simpl in *. intuition; force_specialize_all; solve_rcv.
+  + right. clear IHbal. exists (c::a). solve_rcv.
+    eapply sf_spec.next_ranking_valid. simpl. auto.
+    left. solve_rcv. exists x. exists c. 
+    simpl. auto.
+    exists x. exists c. simpl. auto.
+Qed.
  
     
 Definition boolCmpToProp {A} (c : A -> A -> bool) :=
@@ -745,9 +893,6 @@ induction l; intros.
 Qed.
 
 
-Ltac copy H :=
-match type of H with 
-?P => assert P by exact H end.
 
 Lemma increment_neq' : forall running cd ct  c,
 In (cd, ct) (sf_imp.increment candidate reldec_candidate running c) ->
@@ -1044,8 +1189,8 @@ unfold sf_imp.tabulate in H. destruct (sf_imp.option_split
              (map (sf_imp.next_ranking candidate reldec_candidate rec)
                 election)) eqn:?.
 assert (PRM := insertion_sort_permutation (sf_imp.tabulate' candidate reldec_candidate l)
-                                          (sf_imp.cnlt candidate)).
-rewrite Forall_forall. intros. destruct x. destruct ((sf_imp.insertionsort (sf_imp.cnlt candidate)
+                                          (sf_imp.cnle candidate)).
+rewrite Forall_forall. intros. destruct x. destruct ((sf_imp.insertionsort (sf_imp.cnle candidate)
          (sf_imp.tabulate' candidate reldec_candidate l),
       sf_imp.drop_none l0)) eqn:?. inv H.
 inv Heqp0.
@@ -1074,7 +1219,7 @@ Qed.
 Lemma tabulate_sorted : 
 forall rec election rs election',
 sf_imp.tabulate _ _ rec election = (rs, election') ->
-Sorted (boolCmpToProp (sf_imp.cnlt candidate)) rs.
+Sorted (boolCmpToProp (sf_imp.cnle candidate)) rs.
 Proof.
 intros.
 intros.
@@ -1082,7 +1227,7 @@ unfold sf_imp.tabulate in H. destruct (sf_imp.option_split
              (map (sf_imp.next_ranking candidate reldec_candidate rec)
                 election)) eqn:?.
 inv H. apply insertion_sort_sorted.
-intros. unfold sf_imp.cnlt. destruct b. 
+intros. unfold sf_imp.cnle. destruct b. 
 destruct a. simpl in *. apply leb_false in H.
 apply NPeano.leb_le. auto.
 Qed.
@@ -1220,7 +1365,7 @@ In (cd, ct) (fst (sf_imp.tabulate _ _ r l)).
 Qed.
 
 
-Lemma cnlt_trans : Relations_1.Transitive (boolCmpToProp (sf_imp.cnlt candidate)).
+Lemma cnlt_trans : Relations_1.Transitive (boolCmpToProp (sf_imp.cnle candidate)).
 Proof.
 intro. intros.
 destruct x, y, z.
@@ -1376,7 +1521,7 @@ destruct rs.
                               election)) eqn:?.
              inv Heqp.
              assert (PRM := insertion_sort_permutation ((sf_imp.tabulate'' candidate reldec_candidate l [])) 
-                                                       (sf_imp.cnlt candidate)).
+                                                       (sf_imp.cnle candidate)).
              eapply Permutation_sym in PRM.
              eapply Permutation_in in PRM.
              instantiate (1 := (x, n)) in PRM.
@@ -1464,31 +1609,511 @@ split.
       apply cnlt_trans.
 Qed.
 
-Lemma run_election'_correct : forall fuel election winner tb rec rec',
-    sf_imp.run_election' candidate _ tb election rec fuel = (Some winner, rec') ->
-    sf_spec.winner candidate election (in_record []) winner.
+
+Lemma last_item_in :
+forall l w n,
+sf_imp.last_item candidate l = Some (w,n) ->
+In (w,n) l.
+Proof.
+induction l; intros.
+simpl in *. congruence.
+simpl in *. destruct l. inv H. auto.
+right. auto.
+Qed.
+
+
+
+Lemma tabulate_total_selected : forall r election election' vs,
+sf_imp.tabulate _ _ r election = (vs, election') ->
+sf_spec.total_selected candidate (in_record r) election (length election').
+Proof.
+  intros. unfold sf_imp.tabulate in *.
+  destruct (sf_imp.option_split
+             (map (sf_imp.next_ranking candidate reldec_candidate r) election)) eqn:?.
+  simpl in *. inv H.
+  generalize dependent l0. 
+  revert r  election l.
+  induction election; intros.
+  -   simpl in *. inv Heqp. constructor.
+  - simpl in *. destruct (sf_imp.next_ranking candidate reldec_candidate r a) eqn:?.
+    + repeat dlp. 
+      inv Heqp. simpl in *. apply sf_spec.total_continuing.
+      apply next_ranking_selected in Heqo. 
+      unfold sf_spec.selected_candidate in *. intuition.
+      eapply IHelection. eauto.
+    + dlp. inv Heqp. simpl in *.
+      apply sf_spec.total_exhausted.
+      eapply next_ranking_eliminated; eauto.
+      eapply IHelection; eauto.
+Qed.
+
+Lemma total_selected_unique : forall r e v v',
+sf_spec.total_selected candidate r e v ->
+sf_spec.total_selected candidate r e v' ->
+v= v'.
+Admitted.
+
+Lemma last_item_cons :
+forall h t l,
+sf_imp.last_item candidate (h :: t) = Some l ->
+(t = nil /\ h = l) \/ sf_imp.last_item candidate t = Some l.
+induction t; intros.  
+- simpl in *. inv H. auto.
+- simpl in *. right.
+  auto.
+Qed.
+
+
+Lemma tabulate_not_in : 
+  forall (rec : sf_imp.record candidate)
+         (election : sf_imp.election candidate) (rs : list (candidate * nat))
+         (election' : sf_imp.election candidate) cd,
+    sf_imp.tabulate candidate reldec_candidate rec election = (rs, election') ->
+    ~In cd (fst (split rs)) -> 
+    sf_spec.first_choices candidate (in_record rec) cd election 0.
+Proof.
+intros. 
+eapply tabulate_correct in H. rewrite Forall_forall in H.
+specialize (H (cd, 0)).  simpl in *. apply H.
+Abort. 
+
+Lemma majority_not_0 :
+forall r e x ,
+sf_spec.majority candidate r e x ->
+exists v, sf_spec.first_choices _ r x e v /\ v <> 0.
+Proof.
+intros.
+unfold sf_spec.majority in *.
+edestruct (sf_spec.sf_first_choices_total _ r e x).
+edestruct (sf_spec.total_selected_total _ r e).
+exists x0. intuition.
+subst.
+eapply H in H0; eauto.
+omega.
+Qed.
+
+Lemma ss_last :
+forall l c n,
+StronglySorted (boolCmpToProp (sf_imp.cnle candidate)) l ->
+sf_imp.last_item candidate l = Some (c, n) ->
+Forall (fun (r : candidate * nat) => let (_, y) := r in y <= n) l.
+Proof.
+induction l; intros.
+- simpl in *. intuition.
+- apply last_item_cons in H0.  
+  rewrite Forall_forall; intros.
+  intuition. subst.
+  inv H1. auto. inv H0.
+  inv H.
+  destruct H1.
+  + subst. destruct x. 
+    rewrite Forall_forall in H5.
+    specialize (H5 (c, n)).
+    apply last_item_in in H2. intuition.
+    unfold boolCmpToProp in H.
+    simpl in *.
+    destruct (NPeano.leb n0 n) eqn:?; try contradiction.
+    rewrite NPeano.leb_le in Heqb. auto.
+  + eapply IHl in H2; eauto.
+    rewrite Forall_forall in H2.
+    apply H2.  auto.
+Qed.
+
+Lemma update_eliminated_in_rec : forall rec loser c,
+sf_spec.update_eliminated candidate (in_record rec) loser c <->
+in_record ([loser] :: rec) c.
+Proof.
+split; intros.
+{ induction rec.
+  - unfold sf_spec.update_eliminated in H.
+    intuition. inv H0. destruct H. inv H.
+    subst. unfold in_record. exists [c]. intuition; auto.
+  - unfold sf_spec.update_eliminated in  *. intuition.
+    unfold in_record in H0. destruct H0. intuition.
+    simpl in H2. destruct H2.
+    + subst. unfold in_record. exists x. 
+      intuition.
+    + unfold in_record. exists x. intuition.
+    + unfold in_record in H2. destruct H2.
+      intuition. simpl in H2. destruct H2.
+      * subst. unfold in_record. exists [c].
+        intuition.
+      * exists x. intuition. }
+{ unfold in_record in H. destruct H. intuition. simpl in H0.
+  destruct H0. subst. unfold sf_spec.update_eliminated.
+  right. inv H1; auto. inv H.
+  left. unfold in_record. eauto. }
+Qed.
+
+Axiom prop_ext : forall (P Q : Prop), 
+  (P <-> Q) -> P = Q.
+
+
+Lemma update_eliminated_in_rec_eq : forall rec loser c,
+sf_spec.update_eliminated candidate (in_record rec) loser c =
+in_record ([loser] :: rec) c.
+Proof. intros.
+apply prop_ext. apply update_eliminated_in_rec.
+Qed.
+
+
+Lemma update_eliminated_in_rec_eq_noc : forall rec loser,
+sf_spec.update_eliminated candidate (in_record rec) loser =
+in_record ([loser] :: rec).
+intros. extensionality c. apply update_eliminated_in_rec_eq.
+Qed.
+
+Lemma run_election'_correct : 
+  forall fuel election winner rec' rec tbreak
+         (TB : forall c x, tbreak c = Some x -> In x c) 
+         (N0 : forall c, sf_spec.participates _ c election -> 
+                           sf_spec.first_choices _ (in_record rec) c election 0 ->
+                           in_record rec c),
+    sf_imp.run_election' candidate _ tbreak election rec fuel = (Some winner, rec') ->
+    sf_spec.winner candidate election (in_record rec) winner.
 induction fuel; intros.
 - simpl in *. congruence.
 - simpl in *. destruct (sf_imp.tabulate candidate reldec_candidate rec election) eqn:?; 
                        simpl in *; try congruence.
-  destruct l; try congruence.
+  destruct (sf_imp.last_item candidate l) eqn:?; try congruence.
   destruct p.
-  simpl in *.
-  destruct (sf_imp.gtb_nat n (fst (NPeano.divmod (length e) 1 0 1))) eqn:?.
-  + inv H.f
+  destruct (sf_imp.gtb_nat (n * 2) (length e)) eqn:?.
+  + inv H.
     apply sf_spec.winner_now. unfold sf_spec.majority.
-    intros. 
-Admitted.
+    intros. assert (winner_votes = n).
+    { apply tabulate_correct in Heqp.
+      rewrite Forall_forall in Heqp. specialize (Heqp (winner, n)).
+      apply last_item_in in Heqo. intuition.
+      eapply sf_spec.sf_first_choices_unique in H1; eauto. }
+    subst. 
+    assert (total_votes = (length e)).
+    { apply tabulate_total_selected in Heqp.
+      eapply total_selected_unique; eauto. }
+    subst. 
+    rewrite sf_imp.gtb_nat_gt in Heqb. auto. apply _.
+  + unfold sf_imp.find_eliminated_noopt in *.
+    destruct (tbreak (sf_imp.get_bottom_votes candidate l)) eqn:?. 
+    * rename c0 into loser.
+      rename Heqo0 into TBREAK.
+      copy Heqp. rename H0 into ISLOSER.
+      eapply get_bottom_votes_is_loser in ISLOSER; eauto.
+      rewrite Forall_forall in ISLOSER.
+      eapply TB in TBREAK.
+      apply ISLOSER in TBREAK. 
+      { eapply sf_spec.winner_elimination.
+        - unfold sf_spec.no_majority. 
+          intro. destruct H0.
+          assert (~ sf_spec.majority _ (in_record rec) election c).
+          { intro.
+            unfold sf_spec.majority in *.
+            specialize (H1 (length e) n).
+            copy Heqp.
+            apply tabulate_total_selected in H2. intuition. 
+            apply tabulate_correct in Heqp. 
+            rewrite Forall_forall in Heqp.
+            specialize (Heqp (c, n)). simpl in *.
+            apply last_item_in in Heqo. intuition.
+            rewrite <- sf_imp.gtb_nat_gt in H4. congruence.
+            apply _.
+          }
+          copy Heqp. 
+          apply tabulate_sorted in Heqp.
+          clear - Heqp Heqo H0 H1 H2 N0.
+          destruct (majority_not_0 _ _ _ H0). intuition. 
+          rename H4 into X0. rename H3 into FCX.
+          apply Sorted_StronglySorted in Heqp; [ |  apply cnlt_trans].
+          eapply ss_last in Heqp; eauto.
+          rewrite Forall_forall in *.
+          apply H1. clear H1. intro; intros.
+          assert (winner_votes = n).
+          { apply last_item_in in Heqo.
+            apply tabulate_correct in H2.
+            rewrite Forall_forall in H2. eapply H2 in Heqo; clear H2.
+            eapply sf_spec.sf_first_choices_unique; eauto. }  
+          subst.
+          unfold sf_spec.majority in H0.
+          copy FCX.
+          apply tabulate_first_choices_complete in H3; auto.
+          rewrite H2 in *. simpl in H3.
+          specialize (Heqp (x, x0)).
+          intuition.
+          eapply H0 in FCX; eauto. omega. 
+        - eauto.
+        - rewrite update_eliminated_in_rec_eq_noc.
+          eapply IHfuel.
+          + eauto.
+          + intros. edestruct (rel_dec_p c0 loser).
+            * subst. unfold in_record. exists [loser]. 
+              intuition.
+            * apply N0 in H0. unfold in_record in *. 
+              destruct H0.
+              exists x. intuition.
+              clear - H1 n0.
+             
 
-Lemma tabulate_total_selected : forall r election l election' vs,
-sf_imp.tabulate _ _ r election = (vs, election') ->
-sf_spec.total_selected candidate 
+Lemma first_choices_rec_0 :
+forall c l r e,
+  sf_spec.first_choices candidate (in_record ([l] :: r)) c e 0 ->
+  c <> l ->
+  sf_spec.first_choices candidate (in_record r) c e 0.
+Proof.
+intros.
+inv H. 
+- constructor.
+- constructor. intro. apply H1.
 
+Lemma next_ranking_no_viable : forall a l r  x,
+sf_spec.next_ranking _ (in_record r) a x ->
+sf_spec.no_viable_candidates _ (in_record ([l] :: r)) a ->
+In l x.
+Proof.
+induction a; intros.
+- simpl in *. inv H.
+- simpl in *. intuition.
+  + unfold sf_spec.no_viable_candidates in H0.
+    eapply IHa.
+    eauto. unfold sf_spec.no_viable_candidates. intros.
+    unfold in_record. simpl.
+    specialize (H0 rank). simpl in *. intuition. apply H0 in H3. 
+    unfold in_record in H3.
+    intuition. 
+  + subst. 
+    destruct H. intuition.
+    unfold sf_spec.no_viable_candidates in H0.
+    copy H0.
+    specialize (H a). simpl in H. intuition.
+    copy H1.
+    apply H in H1. 
+    unfold in_record in H1. destruct H1. intuition.
+    simpl in *. intuition. 
+    * subst. assert (x = l). inv H6. auto. inv H1. subst. auto.
+    * clear H4. clear H. unfold in_record in H2. exfalso.
+      apply H2. exists x0. auto.
+Qed.
+
+Lemma still_selected_neq :
+forall c l r a,
+  c <> l ->
+  sf_spec.selected_candidate candidate (in_record r) a c ->
+  sf_spec.selected_candidate candidate (in_record ([l] :: r)) a c.
+Proof.
+  intros.
+  unfold sf_spec.selected_candidate in *.
+  destruct H0. destruct H1. destruct H1.
+  split. 
+  - unfold sf_spec.continuing_ballot in *.
+    intro. apply H0. clear H0.
+    unfold sf_spec.exhausted_ballot in *.
+    assert (In x a). eapply next_ranking_in; eauto.
+    destruct H3. 
+    + assert (In l x).
+      eapply next_ranking_no_viable; eauto.
+      right. unfold sf_spec.overvote. exists x. intuition.
+      exists c. exists l. intuition.
+    + destruct (classic (sf_spec.overvote candidate (in_record r) a)); auto.
+      cut (x = [l]). intros.
+      subst. assert (c = l). inv H2; auto. inv H5. subst. congruence.
+
+Lemma eliminated_overvote_cons :
+forall t r h ,
+Forall r h ->
+sf_spec.overvote candidate r (h :: t) ->
+sf_spec.overvote candidate r t.
+Proof.
+induction t; intros; rewrite Forall_forall in *.
+- destruct H0. destruct H0.
+  destruct H1. destruct H1. intuition. simpl in H0.
+  intuition. subst. destruct H0. intuition.
+- unfold sf_spec.overvote in H0.
+  destruct H0. intuition. destruct H2. destruct H0.
+  intuition. simpl in H1. intuition. 
+  + unfold sf_spec.overvote.
+    exists x. split.
+    simpl. intuition.
+    exists x0. exists x1. intuition.
+  + subst.
+    destruct H5. intuition. clear H1.
+    unfold sf_spec.overvote.  exists a.
+    intuition. simpl. right.
+    intuition. exists x. auto.
+    exists x0. exists x1. auto.
+  + subst.
+    destruct H1. destruct H1.
+    apply H in H1. intuition.
+Qed.
+
+
+Lemma overvote_cons_elim :
+forall h t r,
+(forall c, In c h -> in_record r c) ->
+sf_spec.overvote candidate (in_record r) t ->
+sf_spec.overvote candidate (in_record r) (h :: t).
+intros.
+unfold sf_spec.overvote in *.
+intuitione.
+exists x. intuition.
+simpl. intuition.
+exists x0. exists x1. auto.
+Qed.
+
+Lemma overvote_appears : forall a r x l,
+sf_spec.next_ranking candidate (in_record r) a x ->
+~sf_spec.overvote candidate (in_record r) a ->
+sf_spec.overvote candidate (in_record ([l] :: r)) a ->
+Forall (eq l) x.
+induction a; intros.
+- simpl in *. inv H.
+- simpl in H. destruct H.
+  + destruct H. apply eliminated_overvote_cons in H1; auto.
+    eapply IHa; eauto. intro. apply H0. clear H0. unfold sf_spec.overvote in H3.
+    apply overvote_cons_elim; auto.
+    rewrite Forall_forall. intros.  
+    specialize (H x0). intuition. 
+    clear - H4.
+    unfold in_record in *.
+    intuitione. exists x; simpl; auto.
+  + intuitione. subst.
+    unfold sf_spec.overvote in H1.
+    intuitione.
+    simpl in H1. intuitione.
+    specialize (H1 x0). intuition. unfold in_record in H5. intuitione.
+    simpl in H5. intuition. subst. inv H8.
+    
+
+Lemma not_overvote_not_eliminated :
+forall t r x  a,
+~in_record r x ->
+~sf_spec.overvote candidate (in_record r) (a :: t) ->
+In x a ->
+Forall (eq x) a. 
+induction t; intros.    
+- induction a; intros.
+   + inv H1.
+   + simpl in H1. destruct H1.
+     subst. constructor; auto.
+     eapply IHa. intro. apply H0. clear H0. clear IHa.
+     unfold sf_spec.overvote in *.
+     intuitione. exists (x :: a0).  
+     split. simpl. right. eauto.
+     exists x1. exists x2. simpl in H1. repeat (intuitione; subst).
+     
+     inv H1.
+intuition. 
+     split. simpl in *. destruct H1. intuition.
+     intuitione. subst.
+     right. split.
+     unfold sf_spec.overvote in H0.
+     intuition.
+
+Lemma overvote_cons_and : 
+forall r bal rec, ~sf_spec.overvote candidate rec [x :: x
+     apply IHa.
+
+
+exfalso. apply H0. unfold sf_spec.overvote.
+  exists a. split.
+  + simpl. right.
+    intuition. exists x. auto.
+  + 
+    
+
+
+
+
+exists 
+                               eapply IHa; eauto. intro. apply H0.
+    unfold sf_spec.overvote.
+    unfold sf_spec.overvote in H1. destruct H1.
+    destruct H1. destruct H2. destruct H2. intuition.
+    simpl in H1. simpl in H. intuition.
+  + 
+
+simpl in *. intuition.
+  eapply IHa; eauto.
+unfold sf_spec.overvote in H1.
+destruct H1. destruct H1.
+destruct H2. destruct H2. intuition.
+
+      
+
+
+
+Lemma selected_rec_cons : forall l r a c,
+    c <> l ->
+    sf_spec.selected_candidate candidate (in_record ([l] :: r)) a c ->
+    sf_spec.selected_candidate candidate (in_record r) a c.
+intros.
+unfold sf_spec.selected_candidate in *. intuition. destruct H2. intuition.
+unfold sf_spec.continuing_ballot in *.
+intuition.
+apply H1. unfold sf_spec.exhausted_ballot in *.
+intuition. unfold no_viable_candidates in *. 
+      
+      
+      apply (ClassicalFacts.prop_extensionality _ _ update_eliminated_in_rec) .
+      unfold sf_spec.update_eliminated.
+
+unfold in_record. 
+rewrite <- update_eliminated_in_rec.
+split; intros.
+{ induction rec.
+  - unfold sf_spec.update_eliminated in H.
+    intuition. inv H0. destruct H. inv H.
+    subst. unfold in_record. exists [c]. intuition; auto.
+  - unfold sf_spec.update_eliminated in  *. intuition.
+    unfold in_record in H0. destruct H0. intuition.
+    simpl in H2. destruct H2.
+    + subst. unfold in_record. exists x. 
+      intuition.
+    + unfold in_record. exists x. intuition.
+    + unfold in_record in H2. destruct H2.
+      intuition. simpl in H2. destruct H2.
+      * subst. unfold in_record. exists [c].
+        intuition.
+      * exists x. intuition. }
+{ unfold in_record in H. destruct H. intuition. simpl in H0.
+  destruct H0. subst. unfold sf_spec.update_eliminated.
+  right. inv H1; auto. inv H.
+  left. unfold in_record. eauto. }
+Qed.
+
+Lemma winner_update :
+forall r l w election,
+sf_spec.winner candidate election
+     (sf_spec.update_eliminated candidate (in_record r) l) w
+<->
+sf_spec.winner candidate election
+     (in_record ([l] :: r)) w.
+intros.
+split; intros.
+induction election.
+- inv H. constructor. 
+  unfold sf_spec.majority in *. intros.
+  specialize (H0 total_votes winner_votes).
+  
+
+
+rewrite update_eliminated_in_rec.
+
+exists [c].
+    simpl. intuition. right. left.
+  
+  unfold sf_spec.update_eliminated.
+  eapply IHfuel.
+  unfold sf_imp.find_eliminated_noopt in *.
+  destruct (tbreak (sf_imp.get_bottom_votes candidate l)) eqn:?.
+  eapply get_bottom_votes_is_loser in Heqp; eauto.
+  rewrite Forall_forall in Heqp.
+  apply TB in Heqo0.
+  apply Heqp in Heqo0. apply Heqo0.
+  
+  destruct (
+    
 
 Theorem run_election_correct : forall election winner tb rec, 
     sf_imp.run_election candidate _ tb election = (Some winner, rec) ->
     sf_spec.winner candidate (tb_func_to_Prop tb) election (in_record []) winner.
 intros. unfold sf_imp.run_election in H. apply run_election'_correct in H. auto.
-Qed.y
+Qed.
 
 
